src/Compiler/SeqCompiler.v
@@ -1,0 +1,837 @@
+Require Import String.
+Require Import Vector.
+Require Import DepList.
+Require Import ZArith.
+Require Import GPUCSL.
+Require Import LibTactics.
+Require Import Psatz.
+Require Import Monad.
+Require Import TypedTerm.
+Require Import CUDALib.
+Require Import CSLTactics CodeGen Correctness.
+Require Import mkMap.
+Require Import mkReduce.
+Require Import CodeGenM.
+
+Section codegen.
+  Definition M a := nat -> (a * nat * list cmd).
+
+  Definition bind_M A B (e : M A) (f : A -> M B) : M B:=
+    fun n => let '(v, n, c) := e n in 
+             let '(v', n', c') := f v n in
+             (v', n', c ++ c')%list.
+
+  Definition get : M nat := fun n => (n, n, nil).
+  Definition set n : M unit := fun _ => (tt, n, nil).
+End codegen.
+
+Instance M_monad : Monad M := {ret := fun _ x n => (x, n, nil);
+                               bind := bind_M}.
+
+Definition fresh : M var :=
+  do! n <- get in
+  do! _ <- set (n + 1) in
+  ret (Var (lpref n ++ nat2str 0)).
+
+Definition freshes ty : M (vars ty) :=
+  do! n <- get in
+  do! _ <- set (n + 1) in
+  ret (locals (lpref n) ty 0).
+
+Definition compile_op {t1 t2 t3 : Skel.Typ} (op : Skel.BinOp t1 t2 t3) :=
+  match op in Skel.BinOp t1 t2 t3 return vars t1 -> vars t2 -> exps t3 with
+  | Skel.Eplus => fun e1 e2 => e1 +C e2
+  | Skel.Emult => fun e1 e2 => e1 *C e2
+  | Skel.Eminus => fun e1 e2 => e1 -C e2
+  | Skel.Ediv => fun e1 e2 => e1 /C e2
+  | Skel.Emod => fun e1 e2 => e1 %C e2
+  | Skel.Emin => fun e1 e2 => minC e1 e2
+  | Skel.BEq => fun e1 e2 => Ebinop OP_eq e1 e2
+  | Skel.Blt => fun e1 e2 => Ebinop OP_lt e1 e2
+  end.
+
+Definition setI c : M unit := fun n => (tt, n, c :: nil).
+
+Definition LetE (e : exp) : M var :=
+  do! r <- fresh in
+  do! _ <- setI (r :T Int ::= e) in
+  ret r.
+
+Fixpoint LetEs {ty} : exps ty -> M (vars ty) :=
+  match ty return exps ty -> M (vars ty) with 
+  | Skel.TBool | Skel.TZ => fun e => LetE e
+  | Skel.TTup t1 t2 => fun e => 
+    do! r1 <- LetEs (fst e) in
+    do! r2 <- LetEs (snd e) in
+    ret (r1, r2)
+  end.
+
+Definition Read (le : loc_exp) : M (var) :=
+  do! r <- fresh in 
+  do! _ <- setI (r :T Int ::= [le]) in
+  ret r.
+
+Fixpoint Reads {ty} : lexps ty -> M (vars ty) :=
+  match ty return lexps ty -> M (vars ty) with 
+  | Skel.TBool | Skel.TZ => fun e => Read e
+  | Skel.TTup t1 t2 => fun e => 
+    do! r1 <- Reads (fst e) in
+    do! r2 <- Reads (snd e) in
+    ret (r1, r2)
+  end.
+
+Definition gen_op {t1 t2 t3 : Skel.Typ} (op : Skel.BinOp t1 t2 t3) (x : vars t1) (y : vars t2) : M (vars t3) :=
+  LetEs (compile_op op x y).
+
+Fixpoint ctyps_of_typ (ty : Skel.Typ) :=
+  match ty with
+  | Skel.TBool => Int :: nil
+  | Skel.TZ => Int :: nil
+  | Skel.TTup t1 t2 => (ctyps_of_typ t1 ++ ctyps_of_typ t2)%list
+  end.
+
+Fixpoint nat_of_member {GS : list Skel.Typ} {ty : Skel.Typ}  (mem : member ty GS) : nat :=
+  match mem with
+  | HFirst => 0
+  | HNext m => S (nat_of_member m)
+  end.
+
+Definition seqs := List.fold_right Cseq Cskip.
+
+Lemma safe_seqs_app : forall ntrd BS (tid : Fin.t ntrd) (n : nat) (C1 C2 : list cmd) (s : stack) (h : pheap) (P Q : assn),
+   safe_nt BS tid n (seqs C1) s h P
+   -> (forall s h m, sat s h P -> m <= n -> safe_nt BS tid n (seqs C2) s h Q)
+   -> safe_nt BS tid n (seqs (C1 ++ C2)) s h Q.
+Proof.
+  induction n; [simpl; eauto|].
+  introv.
+  intros (Hskip & Hab1 & Hstep1) Hsafe2; split; [|splits].
+  - Lemma seqs_skip C : seqs C = Cskip -> C = nil.
+    Proof.
+      induction C; simpl; try congruence.
+    Qed.
+    intros Hsk; apply seqs_skip, app_eq_nil in Hsk.
+    destruct Hsk; substs; simpl in Hskip.
+    forwards*: Hskip; forwards*: Hsafe2; simpl in *; jauto.
+  - Lemma seqs_app_abort C1 C2 s h :
+      aborts (seqs (C1 ++ C2)) (s, h)
+      -> aborts (seqs C1) (s, h) \/ (C1 = nil).
+    Proof.
+      induction C1; simpl; eauto.
+      intros Hab; inverts Hab.
+      left; constructor; eauto.
+    Qed.
+    introv Hdis Heq Hab; forwards* [Hab' | ?]: (>>seqs_app_abort Hab); substs.
+    simpl in *; forwards*: Hskip; forwards*: Hsafe2.
+  - Lemma seqs_app_access_ok C1 C2 s h :
+      access_ok (seqs C1) s h 
+      -> (C1 = nil -> access_ok (seqs C2) s h)
+      -> access_ok (seqs (C1 ++ C2)) s h.
+    Proof.
+      induction C1; simpl; eauto.
+    Qed.
+    apply seqs_app_access_ok; jauto.
+    intros; substs; simpl.
+    forwards*: Hskip.
+    forwards*: Hsafe2; simpl in *.
+    jauto.
+  - Lemma seqs_app_write_ok C1 C2 s h :
+      write_ok (seqs C1) s h 
+      -> (C1 = nil -> write_ok (seqs C2) s h)
+      -> write_ok (seqs (C1 ++ C2)) s h.
+    Proof.
+      induction C1; simpl; eauto.
+    Qed.
+    apply seqs_app_write_ok; jauto.
+    intros; substs; simpl.
+    forwards*: Hskip.
+    forwards*: Hsafe2; simpl in *.
+    jauto.
+  - introv Hdis Heq Hstep.
+    Lemma seqs_app_step C1 C2 C' st1 st2 :
+      (seqs (C1 ++ C2)) / st1 ==>s C' / st2
+      -> (exists C'', (seqs C1) / st1 ==>s (seqs C'') / st2 /\ seqs (C'' ++ C2) = C')  \/
+         (C1 = nil).
+    Proof.
+      induction C1; simpl; eauto.
+      intros Hstep; inverts Hstep.
+      - left; exists C1; split; constructor; eauto.
+      - left; exists (c1' :: C1); split; eauto; constructor; eauto.
+    Qed.
+    forwards*[(C' & Hstep' & ?) | ?]: (>>seqs_app_step Hstep); substs; jauto.
+    + destruct Hstep1 as (? & ? & Hstep1 & _).
+      forwards* (h'' & ph' & ? & ?): Hstep1; exists h'' ph'; splits; jauto.
+      applys* IHn; intros; forwards*: (>>Hsafe2 n).
+      applys (>>safe_mon); eauto.
+    + simpl in Hstep.
+      forwards*: Hskip; forwards* (? & ? & Hsafe2'): Hsafe2.
+  - Lemma seqs_app_wait C1 C2 j c:
+      wait (seqs (C1 ++ C2)) = Some (j, c) ->
+      (exists c', c = seqs (c' ++ C2) /\ wait (seqs C1) = Some (j, seqs c')) \/
+      C1 = nil /\ wait (seqs C2) = Some (j, c).
+    Proof.
+      induction C1; simpl. eauto.
+      destruct (wait a) as [[? ?]|]; intros H; inverts H.
+      left; exists (c0 :: C1); eauto.      
+    Qed.
+    intros; forwards*[(c & Hwait & Heq) | [Heq Hwait]]: seqs_app_wait; substs.
+    + destruct Hstep1 as (? & ? & _ & Hstep1).
+      forwards*(phP & ph' & ? & ? & ? & ?): Hstep1.
+      eexists phP, ph'; splits; jauto.
+      intros; applys* IHn; intros; forwards*: Hsafe2.
+      applys* (>>safe_mon).
+    + simpl in H.
+      forwards*: Hskip.
+      forwards* (? & ? & ? & Hsafe2'): Hsafe2.
+Qed.    
+
+Definition gen_if {ty} (b : vars Skel.TBool) (g1 : M (vars ty)) (g2 : M (vars ty)) : M (vars ty) :=
+  fun n => 
+    let '(r1, n, c1) := g1 n in
+    let '(r2, n, c2) := g2 n in
+    let '(res, n, _) := freshes ty n in
+    let c := (Cif (Bunary OP_not (b ==C 0%Z)) 
+                  (seqs c1 ;; assigns res (ty2ctys _) (v2e r1))
+                  (seqs c2 ;; assigns res (ty2ctys _) (v2e r2))) in
+    (res, n, c :: nil).
+
+Fixpoint compile_sexp {GA GS : list Skel.Typ} {typ : Skel.Typ}
+         (se : Skel.SExp GA GS typ) : 
+  hlist (fun ty => var * vars ty)%type GA ->
+  hlist (fun ty => vars ty) GS -> M (vars typ) :=
+  match se with
+  | Skel.EVar _ _ ty v => fun avenv env => LetEs (v2e (hget env v))
+  | Skel.ENum _ _ z => fun avenv env => LetE (Enum z : exps Skel.TZ)
+  | Skel.ELet _ _ t1 t2 e1 e2 => fun avenv env =>
+    do! e1 <- compile_sexp e1 avenv env in
+    compile_sexp e2 avenv (HCons e1 env)
+  | Skel.EBin _ _ _ _ _ op e1 e2 => fun avenv env =>
+    do! x <- compile_sexp e1 avenv env in
+    do! y <- compile_sexp e2 avenv env in
+    gen_op op x y
+  | Skel.EA _ _ typ va e => fun avenv env =>
+    do! i <- compile_sexp e avenv env in
+    let (_, aname) := hget avenv va in
+    Reads (v2gl aname +os i)
+  | Skel.ELen _ _ _ xa => fun avenv env =>
+    let (l, _) := hget avenv xa in LetE (l : exps Skel.TZ)
+  | Skel.EPrj1 _ _ t1 t2 e => fun avenv env =>
+    do! tup <- compile_sexp e avenv env in
+    ret (fst tup)
+  | Skel.EPrj2 _ _ t1 t2 e => fun avenv env =>
+    do! tup <- compile_sexp e avenv env in
+    ret (snd tup)
+  | Skel.ECons _ _ t1 t2 e1 e2 => fun avenv env =>
+    do! r1 <- compile_sexp e1 avenv env in
+    do! r2 <- compile_sexp e2 avenv env in
+    ret (r1, r2)
+  | Skel.EIf _ _ ty e1 e2 e3 => fun avenv env =>
+    do! b <- compile_sexp e1 avenv env in
+    gen_if b (compile_sexp e3 avenv env) (compile_sexp e3 avenv env)
+  end%list.
+
+Instance eq_type_nat : eq_type nat := {eq_dec := eq_nat_dec}.
+
+Fixpoint map_opt {A B : Type} (f : A -> option B) (xs : list A) : option (list B) :=
+  sequence (map f xs).
+
+Definition opt_def {A : Type} (o : option A) d :=
+  match o with
+  | Some x => x
+  | None => d
+  end.
+
+Fixpoint type_of_func (n : nat) :=
+  match n with
+  | O => (cmd * list exp)%type
+  | S n => list var -> type_of_func n
+  end.
+
+Definition evalM {a : Type} (m : M a) (n : nat) : cmd * a :=
+  let '(x, _, c) := m n in (seqs c, x).
+
+Fixpoint dumy_fun_n n x :=
+  match n return type_of_func n with
+  | O => x
+  | S n => fun y => dumy_fun_n n x
+  end.
+
+Definition compile_func {GA fty} (body : Skel.Func GA fty) :
+  AVarEnv GA ->
+  type_of_ftyp fty :=
+  match body in Skel.Func _ fty' return _ -> type_of_ftyp fty' with
+  | Skel.F1 _ _ _ body => fun av xs => evalM (compile_sexp body av (HCons xs HNil)) 0
+  | Skel.F2 _ _ _ _ body => fun av xs ys => evalM (compile_sexp body av (HCons ys (HCons xs HNil))) 0
+  end.
+
+Fixpoint compile_lexp {GA ty} (le : Skel.LExp GA ty) : AVarEnv GA -> exp :=
+  match le in Skel.LExp _ ty return AVarEnv GA -> exp with
+  | Skel.LNum _ n => fun _ => n
+  | Skel.LLen _ _ a => fun aenv => (fst (hget aenv a))
+  | Skel.LMin _ e1 e2 => fun aenv => minC (compile_lexp e1 aenv) (compile_lexp e2 aenv) 
+  end.
+
+Definition accessor_of_array {GA tyxa} aenv (arr : member tyxa GA) :=
+  compile_func (Skel.F1 _ Skel.TZ _ (Skel.EA _ _ _ arr (Skel.EVar _ _ _ HFirst))) aenv.
+
+Definition compile_AE {GA ty} (ae : Skel.AE GA ty) :
+  hlist (fun ty => (var * vars ty))%type GA ->
+  ((var -> (cmd * vars ty))) :=
+  match ae with
+  | Skel.DArr _ _ f len => compile_func f
+  | Skel.VArr _ _ xa => fun avar_env =>
+    let get := accessor_of_array avar_env xa in
+    get
+  end.
+
+Definition compile_AE_len {GA ty}
+           (ae : Skel.AE GA ty) : AVarEnv GA -> exp :=
+  match ae in Skel.AE GA ty return AVarEnv GA -> exp with
+  | Skel.DArr _ _ f len =>
+    fun aenv =>
+    let len' := compile_lexp len aenv in
+    len'
+  | Skel.VArr _ _ xa => fun aenv =>
+    (fst (hget aenv xa))
+  end.
+
+Definition lvar n m := Var (lpref n ++ nat2str m).
+
+Definition fvOk (xs : list var) n : Prop :=
+  List.Forall (fun x => forall m k, x = lvar m k -> m < n) xs.
+
+Lemma fvOk_weaken fvs n m :
+  n <= m -> fvOk fvs n -> fvOk fvs m.
+Proof.
+  unfold fvOk; intros Hnm H; induction H; constructor; eauto.
+  intros; forwards*: H; omega.
+Qed.
+
+Lemma fvOk_ge n m k xs :
+  fvOk xs n -> n <= m -> ~ In (lvar m k) xs.
+Proof.
+  unfold fvOk; rewrite Forall_forall; intros H ? Hc.
+  intros; forwards*: H; omega.
+Qed.
+
+Lemma fvOk_incl xs ys n :
+  fvOk xs n -> incl ys xs -> fvOk ys n.
+Proof. unfold fvOk; eauto using Forall_incl. Qed.
+
+Lemma fvOk_app xs ys n : fvOk xs n -> fvOk ys n -> fvOk (xs ++ ys) n. 
+Proof. applys* Forall_app. Qed.
+
+Definition assnInv (P : assn) : nat -> Prop := 
+  fun n => (exists xs, fv_assn P xs /\ fvOk xs n).
+
+Definition assnOk (P : assn) (C : cmd) (Q : assn) :=
+  forall ntrd BS tid, @CSL ntrd BS tid P C Q.
+
+Definition Gsat {T} (P : assn) (gen : M T) (Q : T -> assn) :=
+  forall n n' c v,
+    assnInv P n 
+    -> gen n = (v, n', c) 
+    -> n <= n' /\ assnInv (Q v) n' /\ assnOk P (seqs c) (Q v).
+
+Lemma rule_app_seqs ntrd BS (tid : Fin.t ntrd) P Q R st1 st2 :
+  CSL BS tid P (seqs st1) Q
+  -> CSL BS tid Q (seqs st2) R
+  -> CSL BS tid P (seqs (st1 ++ st2)) R.
+Proof.
+  unfold CSL; intros H1 H2; intros.
+  applys* safe_seqs_app.
+Qed.
+
+Lemma rule_bind_c T U P (gen : M T) (gen' : T -> M U) Q R :
+  Gsat P gen Q
+  -> (forall v, Gsat (Q v) (gen' v) R)
+  -> Gsat P (bind gen gen') R.
+Proof.
+  unfold Gsat, assnInv, bind, ret; simpl; unfold bind_M; simpl.
+  intros Hgen Hgen' n n' c v v' Heq.
+  destruct (gen n) as [[_v _n] _c] eqn:Heq1.
+  destruct (gen' _v _n) as [[_v' _n'] _c'] eqn:Heq2.
+  inverts Heq.
+  forwards*(? & (? & ? & ?) & ?): Hgen.
+  forwards*(? & (? & ? & ?) & ?): Hgen'.
+  splits; [omega|eexists; splits|]; jauto.
+  unfold assnOk; intros; applys* rule_app_seqs.
+Qed.
+
+Lemma rule_backward_c T P (gen : M T) Q Q' :
+  Gsat P gen Q
+  -> (forall v, Q v |= Q' v)
+  -> (forall v xs, fv_assn (Q v) xs -> fv_assn (Q' v) xs)
+  -> Gsat P gen Q'.
+Proof.
+  unfold Gsat, assnInv, assnOk; introv ? ? ? ? ?.
+  forwards*(? & (xs & ? & ?) & ?): H; splits; [omega|exists xs; splits*|].
+  intros; eapply forward; [|eauto]; eauto.
+Qed.
+
+Lemma string_app_assoc a b c : ((a ++ b) ++ c = a ++ b ++ c)%string.
+Proof.
+  induction a; simpl; congruence.
+Qed.
+
+Definition char a := String a EmptyString.
+Definition str_in s c := exists s1 s2, s = (s1 ++ char c ++ s2)%string.
+
+Lemma sep_var_inj s1 s1' c s2 s2' :
+  (s1 ++ char c ++ s2 = s1' ++ char c ++ s2')%string ->
+  ~str_in s1 c -> ~str_in s1' c ->
+  s1 = s1'.
+Proof.
+  revert s1' s2 s2'; induction s1; simpl; introv Heq Hin Hin'.
+  - destruct s1'; simpl in *; eauto.
+    assert (c <> a).
+    { intros Hc; substs.
+      apply Hin'.
+      exists EmptyString (s1'); eauto. }
+    inverts Heq; congruence.
+  - destruct s1'; simpl in *; inverts Heq.
+    { false; apply Hin; exists EmptyString s1; eauto. }
+    forwards*: (>>IHs1 s1'); try congruence.
+    { intros (t1 & t2 & Heq'); apply Hin; exists (char a0 ++ t1)%string t2; simpl in *; congruence. }
+    { intros (t1 & t2 & Heq'); apply Hin'; exists (char a0 ++ t1)%string t2; simpl in *; congruence. }
+Qed.
+
+Definition char_of_string s := match s with
+                               | String c _ => c
+                               | _ => Ascii.zero
+                               end.
+
+Lemma nat_to_str_underbar n :
+  ~str_in (nat2str n) (char_of_string "_").
+Proof.
+  induction n; simpl; intros (s1 & s2 & Heq).
+  - destruct s1; simpl in *; try congruence.
+    inverts Heq.
+    destruct s1; simpl in *; try congruence.
+  - destruct s1; simpl in *; try congruence.
+    inverts Heq.
+    apply IHn; exists s1 s2; eauto.
+Qed.
+
+Lemma lpref_inj a b c d : (lpref a ++ b = lpref c ++ d -> a = c /\ b = d)%string.
+Proof.
+  unfold lpref; intros H.
+  inverts H as Heq.
+  forwards*: (sep_var_inj (nat2str a) (nat2str c)); simpl in *; eauto using nat_to_str_underbar.
+  rewrite !string_app_assoc in Heq; simpl in *; eauto.
+  forwards*: (>>nat_to_string_inj H); split; eauto.
+  substs; apply string_inj2 in Heq; eauto.
+Qed.      
+
+Lemma evar_inj x y : Var x = Var y -> x = y. intros H; inverts* H. Qed.
+
+Lemma fvOk_locals n m k ty :
+  n < m
+  -> fvOk (flatTup (locals (lpref n) ty k)) m.
+Proof.
+  revert k; induction ty; intros; [
+    constructor; eauto; 
+    introv Heq; apply evar_inj in Heq; forwards*(? & ?): (>>lpref_inj Heq); 
+    omega..|].
+  simpl; apply fvOk_app; eauto.
+Qed.
+
+Lemma rule_fLet_s R P E (e : exp) v :
+  evalExp E e v
+  -> Gsat (Assn R P E)
+          (LetE e)
+          (fun x => (Assn R P (x |-> v :: E))).
+Proof.
+  unfold Gsat, assnInv, assnOk, LetE, bind; simpl; unfold bind_M; simpl.
+  introv Heval Hfv Heq; inverts Heq.
+  splits; [omega|intros..].
+  - destruct Hfv as (xs & ? & ?); exists (Var (lpref n ++ nat2str 0)%string :: xs); splits.
+    rewrite fv_assn_base_eq in *; simpl.
+    apply incl_cons_lr; eauto.
+    constructor; [|eapply fvOk_weaken; [|eauto]; omega].
+    introv Heq.
+    apply evar_inj, lpref_inj in Heq; omega.
+  - eapply rule_seq.
+    apply rule_assign; eauto.
+    eapply backward; [|apply rule_skip].
+    prove_imp.
+    rewrite remove_var_disjoint; eauto.
+    destruct Hfv as (xs & ? & ?).
+    apply fv_assn_base_eq in H3.
+    intros Hin.
+    forwards*: H3.
+    unfold fvOk in H4. 
+    rewrite List.Forall_forall in H4.
+    forwards*: (>>H4 H5 n 0).
+    omega.
+Qed.
+
+Lemma rule_ret_s T (v : T) P Q :
+  (P |= Q v)
+  -> (forall xs, fv_assn P xs -> fv_assn (Q v) xs)
+  -> Gsat P (ret v) Q.
+Proof.
+  unfold Gsat, assnInv, assnOk; introv ? ? ? Heq.
+  inverts Heq.
+  forwards* (xs & ? & ?): H1.
+  splits; [omega|exists xs; splits*|].
+  intros; eapply forward; [|apply rule_skip]; eauto.
+Qed.
+
+Lemma rule_fLets_s' ty R P E (e : exps ty) v E' :
+  evalExps E e v
+  -> Gsat (Assn R P (E' ++ E))
+          (LetEs e)
+          (fun x => (Assn R P (x |=> v ++ (E' ++ E)))).
+Proof.
+  revert E'; induction ty; intros; try now (apply rule_fLet_s; applys* evalExp_app_ig).
+  inverts H.
+  simpl.
+  eapply rule_bind_c.
+  applys* IHty1.
+  introv.
+  eapply rule_bind_c.
+  rewrite app_assoc.
+  applys* IHty2.
+  intros.
+  apply rule_ret_s.
+  prove_imp.
+  introv; rewrite! fv_assn_base_eq; rewrite <-!app_assoc, !map_app.
+  unfold incl; intros H a; specialize (H a); rewrite !in_app_iff in *; intuition.
+Qed.
+
+Lemma rule_fLets_s ty R P E (e : exps ty) v :
+  evalExps E e v
+  -> Gsat (Assn R P E)
+          (LetEs e)
+          (fun x => (Assn R P (x |=> v ++ E))).
+Proof. 
+  intros.
+  apply (rule_fLets_s' _ _ _ _ _ _ (@nil entry)); jauto.
+Qed.
+
+Lemma rule_Read_s R R' (P : Prop) E p l le v :
+  evalLExp E le l
+  -> (P -> R |=R l |->p (p, v) *** R')
+  -> Gsat (Assn R P E)
+          (Read le)
+          (fun x => (Assn R P (x |-> v :: E))).
+Proof.
+  unfold Gsat, assnInv, assnOk, LetE, bind; simpl; unfold bind_M; simpl.
+  introv Heval Hres Hfv Heq; inverts Heq.
+  splits; [omega|intros..].
+  - destruct Hfv as (xs & ? & ?); exists (Var (lpref n ++ nat2str 0)%string :: xs); splits.
+    rewrite fv_assn_base_eq in *; simpl.
+    apply incl_cons_lr; eauto.
+    constructor; [|eapply fvOk_weaken; [|eauto]; omega].
+    introv Heq.
+    apply evar_inj, lpref_inj in Heq; omega.
+  - eapply rule_seq.
+    applys* rule_read; eauto.
+    eapply backward; [|apply rule_skip].
+    prove_imp.
+    rewrite remove_var_disjoint; eauto.
+    destruct Hfv as (xs & ? & ?).
+    apply fv_assn_base_eq in H3.
+    intros Hin.
+    forwards*: H3.
+    unfold fvOk in H4. 
+    rewrite List.Forall_forall in H4.
+    forwards*: (>>H4 H5 n 0).
+    omega.
+Qed.
+
+Lemma rule_Reads_s' ty R R' (P : Prop) E E' p l (le : lexps ty) v :
+  evalLExps E le l
+  -> (P -> R |=R l |=>p (p, v) *** R')
+  -> Gsat (Assn R P (E' ++ E))
+          (Reads le)
+          (fun x => (Assn R P (x |=> v ++ (E' ++ E)))).
+Proof.
+  revert E' R'; induction ty; intros; try now (applys* rule_Read_s; applys* evalLExp_app_ig).
+  inverts H.
+  simpl.
+  eapply rule_bind_c.
+  applys* IHty1.
+  simpl in H0.
+  intros; forwards*: H0.
+  rewrite <-res_assoc in H4; apply H4.
+  introv.
+  eapply rule_bind_c.
+  rewrite app_assoc.
+  applys* IHty2.
+  simpl in H0; intros; forwards*: H0.
+  rewrite <-res_assoc, res_CA in H4; apply H4.
+  intros.
+  apply rule_ret_s.
+  prove_imp.
+  introv; rewrite! fv_assn_base_eq; rewrite <-!app_assoc, !map_app.
+  unfold incl; intros H a; specialize (H a); rewrite !in_app_iff in *; intuition.
+Qed.
+
+Lemma rule_Reads_s ty R R' (P : Prop) E p l (le : lexps ty) v :
+  evalLExps E le l
+  -> (P -> R |=R l |=>p (p, v) *** R')
+  -> Gsat (Assn R P E)
+          (Reads le)
+          (fun x => (Assn R P (x |=> v ++ E))).
+Proof.
+  intros; eapply (rule_Reads_s' _ _ _ _ _ nil); eauto.
+Qed.
+
+Lemma incl_app_iff A (xs ys zs : list A) :
+  incl (xs ++ ys) zs <-> incl xs zs /\ incl ys zs.
+Proof.
+  split.
+  - induction xs; intros; splits; eauto using incl_nil_l.
+    intros x Hin; specialize (H x); simpl in *; rewrite in_app_iff in *; eauto.
+    apply H; destruct Hin; eauto.
+    forwards*: IHxs.
+    intros x Hin; specialize (H x); simpl in *; rewrite in_app_iff in *; eauto.
+  - intros; apply incl_app; jauto.
+Qed.
+
+Lemma rule_gen_if ty R P E (b : var) v v1 v2 (g1 : M (vars ty)) g2 R1 R2 P1 P2 E1 E2 :
+  evalExp E b v
+  -> Gsat (Assn R (P /\ (v <> 0%Z)) E) g1 (fun x => Assn R1 P1 (x |=> v1 ++ E1))
+  -> Gsat (Assn R (P /\ (v = 0%Z)) E) g2 (fun x => Assn R2 P2 (x |=> v2 ++ E2))
+  -> Gsat (Assn R P E) (gen_if b g1 g2) (fun x => Assn R1 P1 (x |=> v1 ++ E1) \\// Assn R2 P2 (x |=> v2 ++ E2) ).
+Proof.
+  unfold Gsat, assnInv, assnOk, gen_if; introv Heval Hgen1 Hgen2 Hfv Heq.
+  destruct (g1 n) as [[r1 n1] c1] eqn:Heq1.
+  destruct (g2 n1) as [[r2 n2] c2] eqn:Heq2.
+  destruct (freshes ty n2) as [[res n3] ?] eqn:Heq3.
+  inverts Heq.
+  forwards (xs & ? & ?): Hfv.
+  forwards*(? & (xs1 & ? & ?) & ?): Hgen1; [exists xs; splits; jauto|].
+  rewrites* fv_assn_base_eq in *.
+  forwards*(? & (xs2 & ? & ?) & ?): Hgen2.
+  exists xs; splits.
+  rewrites* fv_assn_base_eq in *.
+  eapply fvOk_weaken; [|eauto]; omega.
+  unfold freshes, bind in *; simpl in *; unfold bind_M in *; simpl in *.
+  inverts Heq3.
+  splits; [omega|..].
+  - exists (flatTup (locals (lpref n2) ty 0) ++ xs1 ++ xs2).
+    rewrite fv_assn_disj_eq.
+    splits.
+    exists (flatTup (locals (lpref n2) ty 0) ++ xs1) (flatTup (locals (lpref n2) ty 0) ++ xs2).
+    splits; [rewrite !fv_assn_base_eq, map_app, map_flatTup, incl_app_iff in *; 
+              splits; [apply incl_appl|apply incl_appr]; jauto..|].
+    intros x; rewrite !in_app_iff; splits; [intros [?|[?|?]]|intros [[? | ?]|[? | ?]]]; jauto.
+    repeat apply fvOk_app.
+    apply fvOk_locals; omega.
+    eapply fvOk_weaken; [|eauto]; omega.
+    eapply fvOk_weaken; [|eauto]; omega.
+  - intros.
+    eapply rule_seq.
+    { eapply rule_if_disj; [do 2 constructor; eauto; constructor|..].
+      - eapply rule_seq; [eauto|].
+        eapply forwardR; [eapply rule_assigns|].
+        { rewrite fvEs_v2e.
+          rewrite fv_assn_base_eq, map_app, incl_app_iff in H2.
+          apply not_in_disjoint.
+          intros ? ? ?.
+          apply locals_pref in H9 as (? & ? & ?); substs.
+          destruct H2 as [Hin ?].
+          rewrite map_flatTup in Hin; apply Hin in H10.
+          unfold fvOk in H3; rewrite Forall_forall in H3.
+          forwards*: (>>H3 H10).
+          omega. }
+        { apply locals_disjoint_ls. }
+        { evalExps. }
+        rewrites remove_vars_disjoint; [eauto|].
+        apply not_in_disjoint; intros x ? ?.
+        rewrite fv_assn_base_eq in H2; forwards*: H2.
+        apply locals_pref in H10 as (? & ? & ?); substs.
+        unfold fvOk in H3; rewrite Forall_forall in H3; forwards*: (>>H3 H11); omega.
+      - eapply rule_seq; [simpl; eauto|].
+        eapply backward.
+        { instantiate (1 := Assn R (P /\ v = 0%Z) E).
+          prove_imp. }
+        eauto.
+        eapply forwardR; [eapply rule_assigns|].
+        { rewrite fvEs_v2e.
+          rewrite fv_assn_base_eq, map_app, incl_app_iff in H6.
+          apply not_in_disjoint.
+          intros ? ? ?.
+          apply locals_pref in H9 as (? & ? & ?); substs.
+          destruct H6 as [Hin ?].
+          rewrite map_flatTup in Hin; apply Hin in H10.
+          unfold fvOk in H7; rewrite Forall_forall in H7.
+          forwards*: (>>H7 H10).
+          omega. }
+        { apply locals_disjoint_ls. }
+        { evalExps. } 
+        rewrites remove_vars_disjoint; [eauto|].
+        apply not_in_disjoint; intros x ? ?.
+        rewrite fv_assn_base_eq in H6; forwards*: H6.
+        apply locals_pref in H10 as (? & ? & ?); substs.
+        unfold fvOk in H7; rewrite Forall_forall in H7; forwards*: (>>H7 H11); omega. }
+    eapply forward; [|apply rule_skip].
+    intros s h [Hsat|Hsat]; fold_sat_in Hsat; [left | right]; fold_sat; revert s h Hsat; prove_imp.
+    all: rewrites remove_vars_disjoint; [rewrite in_app_iff; eauto|].
+Qed.
+
+Require Import Program.
+
+Lemma scInv_incl GS e (svar_env : SVarEnv GS) seval_env ty (m : member ty GS) :
+  In e ((hget svar_env m) |=> sc2CUDA (hget seval_env m)) ->
+  In e (scInv svar_env seval_env).
+Proof.
+  unfold scInv; induction GS; simpl in *;
+  dependent destruction m; dependent destruction svar_env; dependent destruction seval_env;
+  simpl in *; rewrite in_app_iff; eauto.
+Qed.
+
+Ltac prove_fv_assn := 
+  repeat first [rewrite fv_assn_base_eq | 
+                rewrite map_app |
+                rewrite incl_app_iff|
+                rewrite map_flatTup]; jauto.
+
+Lemma compileExp_ok E ty1 ty2 ty3 (op : Skel.BinOp ty1 ty2 ty3) v1 (x1 : vars ty1) v2 (x2 : vars ty2) :
+  evalExps E (v2e x1) (sc2CUDA v1)
+  -> evalExps E (v2e x2) (sc2CUDA v2)
+  -> evalExps E (compile_op op x1 x2) (sc2CUDA (Skel.opDenote _ _ _ op v1 v2)).
+Proof.
+  induction op; simpl; intros; try (econstructor; eauto).
+  equates 1; [econstructor; eauto|]; simpl.
+  destruct (Z.eqb_spec v1 v2), eq_dec; omega.
+  equates 1; [econstructor; eauto|]; simpl.
+  destruct (Z.ltb_spec v1 v2), Z_lt_dec; omega.
+Qed.
+
+Lemma aname_eval GA (avar_env : AVarEnv GA) (aptr_env : APtrEnv GA) (aeval_env : AEvalEnv GA)
+      ty (m : member ty GA) len aname :
+  hget avar_env m = (len, aname) ->
+  evalLExps (arrInvVar avar_env aptr_env aeval_env) (v2gl aname) (val2gl (hget aptr_env m)).
+Proof.
+  unfold arrInvVar; induction GA;
+  dependent destruction m;
+  dependent destruction avar_env;
+  dependent destruction aptr_env; 
+  dependent destruction aeval_env; simpl; intros; substs.
+  
+  apply evalLExps_gl.
+
+  apply evalExps_vars.
+  repeat rewrite <-app_assoc; simpl.
+  apply incl_cons_ig.
+  apply incl_appl; eauto.
+  
+  destruct p; simpl.
+
+  apply evalLExps_cons_ig, evalLExps_app_ig; eauto.
+Qed.
+
+Require Import SetoidClass.
+
+Lemma arrInvRes_unfold GA (aptr_env : APtrEnv GA) (aeval_env : AEvalEnv GA)
+      ty (m : member ty GA) p :
+  exists R,
+        (arrInvRes aptr_env aeval_env p ==
+        (arrays (val2gl (hget aptr_env m)) (arr2CUDA (hget aeval_env m)) p *** R))%type.
+Proof.
+  unfold arrInvRes; induction GA; 
+  dependent destruction m;
+  dependent destruction aptr_env;
+  dependent destruction aeval_env; simpl.
+  - eexists; reflexivity.
+  - forwards*(R & Heq): (>>IHGA m).
+    eexists.
+    rewrite Heq.
+    rewrite res_CA.
+    reflexivity.
+Qed.
+
+Lemma nth_error_lt' A (arr : list A) i v : 
+  List.nth_error arr i = Some v -> i < length arr.
+Proof.
+  revert i v; induction arr; intros i v; destruct i; simpl; inversion 1; try omega.
+  forwards*: IHarr; omega.
+Qed.
+
+Lemma nth_error_lt A (arr : list A) i v : 
+  SkelLib.nth_error arr i = Some v -> (0 <= i /\ i < SkelLib.len arr)%Z.
+Proof.
+  unfold SkelLib.nth_error, SkelLib.Z_to_nat_error.
+  destruct Z_le_dec; try now inversion 1.
+  unfold ret; simpl; unfold bind_opt.
+  intros H; apply nth_error_lt' in H.
+  rewrite Nat2Z.inj_lt in H.
+  rewrite !Z2Nat.id in H; unfold SkelLib.len; omega.
+Qed.
+
+Lemma nth_error_lt_nat A (arr : list A) i v : 
+  SkelLib.nth_error arr i = Some v
+  -> exists i', Zn i' = i /\ (0 <= i' /\ i' < length arr).
+Proof.
+  intros; exists (Z.to_nat i).
+  forwards*: nth_error_lt.
+  rewrites Z2Nat.id; [|lia].
+  unfold SkelLib.len in *.
+  zify; rewrite Z2Nat.id in *; [|lia..].
+  lia.
+Qed.
+
+Lemma compile_sexpOk (GA GS : list Skel.Typ) (typ : Skel.Typ)
+      (se : Skel.SExp GA GS typ) 
+      (svenv : SVarEnv GS)
+      (seenv : SEvalEnv GS)
+      (avenv : AVarEnv GA)
+      (apenv : APtrEnv GA)
+      (aeenv : AEvalEnv GA) p resEnv v R P :
+  Skel.sexpDenote GA GS typ se aeenv seenv = Some v ->
+  Gsat (sexpInv svenv seenv avenv apenv aeenv R P resEnv p)
+       (compile_sexp se avenv svenv)
+       (fun es => sexpInv svenv seenv avenv apenv aeenv R P (es |=> sc2CUDA v ++ resEnv) p).
+Proof.
+  unfold sexpInv.
+  revert typ v se seenv svenv R P resEnv.
+  induction se; introv Heval; inverts Heval; simpl.
+  - eapply rule_backward_c.
+    apply rule_fLets_s.
+    { apply evalExps_vars.
+      apply incl_appr, incl_appl.
+      unfold incl; intros; eauto using scInv_incl. }
+    { simpl; intros ?; prove_imp. }
+    introv. 
+    prove_fv_assn.
+  - eapply rule_backward_c.
+    apply rule_fLet_s.
+    { evalExp. }
+    { simpl; intros ?; prove_imp. }
+    introv; simpl.
+    prove_fv_assn.
+  - destruct (Skel.sexpDenote _ _ _ se1 _ _) eqn:Heq1; [|inverts H0].
+    destruct (Skel.sexpDenote _ _ _ se2 _ _) eqn:Heq2; [|inverts H0].
+    inverts H0.
+    eapply rule_bind_c; eauto.
+    introv.
+    eapply rule_bind_c; eauto.
+    introv.
+    eapply rule_backward_c.
+    { apply rule_fLets_s.
+      apply compileExp_ok; evalExps. }
+    + simpl; intros ?; prove_imp.
+    + introv; prove_fv_assn.
+  - destruct (Skel.sexpDenote _ _ _ se _ _) eqn:Heq1; [|inverts H0].
+    forwards*(R' & Heq'): (>> arrInvRes_unfold apenv aeenv m p).
+    unfold bind in H0; simpl in H0.    
+    forwards*(i & ? & ?): nth_error_lt_nat.
+    eapply rule_bind_c; eauto.
+    introv; simpl.
+    destruct (hget avenv m) as [alen aname] eqn:Heq.
+    eapply rule_backward_c.
+    eapply rule_Reads_s.
+    { apply eval_locs_off; [|evalExp].
+      apply evalLExps_cons_ig, evalLExps_app_ig, evalLExps_app_ig. 
+      applys* aname_eval. }
+    intros.
+    rewrite Heq' in H3.
+    rewrites (>>arrays_unfold i) in H3.
+    { unfold arr2CUDA; rewrite map_length; omega. }
+    rewrite <-!res_assoc in *.
+    rewrite res_CA in H3; apply H3.
+    intros ?; simpl; prove_imp.
